fix lemmas for exponent blinding

specs/experimental/Spec.RSA.Lemmas.fst
@@ -9,17 +9,17 @@ type elem (n:nat) = e:nat{e < n}
 #reset-options "--z3rlimit 30 --max_fuel 2"
 val pow : x:nat -> n:nat -> Tot nat
 let rec pow x n =
-  match n with
-  | 0 -> 1
-  | n -> x * pow x (n - 1)
+    match n with
+    | 0 -> 1
+    | n -> x * pow x (n - 1)
 
 val lemma_pow: x:nat -> n:nat -> m:nat -> Lemma
-  (pow x n * pow x m = pow x (n + m))
+    (pow x n * pow x m = pow x (n + m))
 let rec lemma_pow x n m =
-  let ass (x y z : nat) : Lemma ((x*y)*z == x*(y*z)) = () in
-  match n with
-  | 0 -> ()
-  | _ -> lemma_pow x (n-1) m; ass x (pow x (n-1)) (pow x m)
+    let ass (x y z : nat) : Lemma ((x*y)*z == x*(y*z)) = () in
+    match n with
+    | 0 -> ()
+    | _ -> lemma_pow x (n-1) m; ass x (pow x (n-1)) (pow x m)
 
 val lemma_pow_greater_0: a:nat{a > 0} -> b:nat -> Lemma
 	(requires True)
@@ -56,13 +56,15 @@ let lemma_pow_mul a b c = admit()
 
 val lemma_pow_div:
     a:nat -> b:nat -> d:nat{d > 0} -> Lemma
-    (pow (a / d) b == (pow a b) / pow d b)
+    (pow (a / d) b = (pow a b) / pow d b)
 let lemma_pow_div a b d = admit()
 
 val lemma_pow_a2_b:
-	a:nat -> b:nat -> Lemma 
+	a:nat -> b:nat -> Lemma
     (pow (a * a) b = pow a (2 * b))
-let lemma_pow_a2_b a b = admit()
+let lemma_pow_a2_b a b =
+    lemma_pow_mul a a b;
+    lemma_pow a b b
 
 val lemma_pow_mod:
 	a:nat -> b:nat -> n:pos -> Lemma 
@@ -77,8 +79,12 @@ let lemma_mod_mult_div_1 a d n = admit()
 val lemma_mod_mult_div:
     a:nat -> b:nat -> d:nat{d > 0} -> n:nat{n > 0} -> Lemma
     ((a * b / d) % n == ((a % n) * b / d) % n)
-let lemma_mod_mult_div a b d n = admit()
+let lemma_mod_mult_div a b d n =
+    lemma_mod_mult_div_1 (a * b) d n;
+    lemma_mod_mul_distr_l a b n;
+    lemma_mod_mult_div_1 ((a % n) * b) d n
 
+// (1 / d) % n is an inverse element of d
 val lemma_mult_div_mod:
     a:nat -> b:nat -> d:nat{d > 0} -> n:nat{n > 0} -> Lemma
     ((a * (b / d)) % n == (a * b / d) % n)
@@ -89,69 +95,12 @@ val lemma_div_lt_ab: a:nat -> b:nat -> d:pos -> Lemma
     (ensures (a / d < b / d))
 let lemma_div_lt_ab a b d = admit()
 
-(* LEMMAS for exponent blinding *)
-val lemma_mod_pq:
-	a:nat -> b:nat -> p:nat{p > 1} -> q:nat{q > 1} -> Lemma
-	(requires (a % p == b /\ a % q == b))
-	(ensures (a % (p * q) == b))
-let lemma_mod_pq a b p q = admit()
-
-// m ^ (p - 1) = 1 (mod p) where m is any integer and p is a prime number
-val fermat_little_theorem:
-	p:nat{p > 1} -> m:nat{m > 0} -> Lemma
-    ((pow m (p - 1)) % p == 1)
-let fermat_little_theorem p m = admit()
-
-#reset-options "--z3rlimit 50 --max_fuel 0"
-
-val lemma_exp_blinding_1:
-	n:nat{n > 1} -> phi_n:nat -> p:elem n{p > 1} ->
-	q:elem n{q > 1} -> m:elem n{m > 0} -> Lemma
-	(requires (phi_n == (p - 1) * (q - 1) /\ n = p * q))
-	(ensures ((pow m phi_n) % q == 1))
-let lemma_exp_blinding_1 n phi_n p q m =
-	lemma_pow_pow m (q - 1) (p - 1);
-	lemma_pow_mod (pow m (q - 1)) (p - 1) q;
-	fermat_little_theorem q m;
-	lemma_pow_1 (p - 1);
-	assert ((pow m phi_n) % q == 1)
-
-val lemma_exp_blinding_2:
-	n:nat{n > 1} -> phi_n:nat -> p:elem n{p > 1} ->
-	q:elem n{q > 1} -> m:elem n{m > 0} -> Lemma
-	(requires (phi_n == (p - 1) * (q - 1) /\ n = p * q))
-	(ensures ((pow m phi_n) % (p * q) == 1))
-let lemma_exp_blinding_2 n phi_n p q m =
-	lemma_exp_blinding_1 n phi_n p q m;
-	lemma_exp_blinding_1 n phi_n q p m;
-	lemma_mod_pq (pow m phi_n) 1 p q
-
-#reset-options "--z3rlimit 150 --max_fuel 0"
-
-val lemma_exp_blinding:
-	n:nat{n > 1} -> phi_n:nat -> p:elem n{p > 1} -> q:elem n{q > 1} ->
-	d:elem n{d > 0} -> d':nat -> m:elem n{m > 0} -> r:nat -> Lemma
-	(requires (phi_n = (p - 1) * (q - 1) /\ n = p * q /\ d' = d + r * phi_n))
-	(ensures ((pow m d') % n  == (pow m d) % n))
-let lemma_exp_blinding n phi_n p q d d' m r =
-    let res:nat = (pow m d') % n in
-	lemma_pow m d (r * phi_n);
-	lemma_pow_pow m phi_n r;
-	lemma_pow_mod (pow m phi_n) r n;
-	assert ((pow (pow m phi_n) r) % n == (pow ((pow m phi_n) % n) r) % n);
-    lemma_exp_blinding_2 n phi_n p q m;
-    assert ((pow m phi_n) % (p * q) == 1);
-    assert ((pow (pow m phi_n) r) % n == (pow 1 r) % n);
-	lemma_pow_1 r;
-	modulo_lemma 1 n;
-	lemma_mod_mul_distr_l (pow m (r * phi_n)) (pow m d) n
-
 (* LEMMAS for Karatsuba's multiplication *)
 val lemma_distributivity_mult: a:int -> b:int -> c:int -> d:int -> Lemma
   ((a + b) * (c + d) = a * c + a * d + b * c + b * d)
 let lemma_distributivity_mult a b c d = ()
 
-#reset-options "--z3rlimit 50 --initial_fuel 0 --max_fuel 0"
+#reset-options "--z3rlimit 150 --initial_fuel 0 --max_fuel 0"
 
 val lemma_karatsuba_mult:
 	x:nat -> a:nat -> a0:nat -> a1:nat ->
@@ -194,14 +143,14 @@ val abs: x:int -> Tot (y:int{ (x >= 0 ==> y = x) /\ (x < 0 ==> y = -x) })
 let abs x = if x >= 0 then x else -x
 
 (* LEMMAS for Montgomery's arithmetic *)
+#reset-options "--z3rlimit 50 --max_fuel 0"
 val lemma_mod_div_simplify: a:nat -> r:nat{r > 0} -> n:nat{n > 0} -> Lemma
   (((a * ((r * r) % n)) / r) % n == (a * r) % n)
 let lemma_mod_div_simplify a r n =
     let res : nat = ((a * ((r * r) % n)) / r) % n in
     lemma_mod_mult_div (r * r) a r n;
-    assert (res == ((a * r * r) / r) % n);
+    paren_mul_right a r r;
     paren_mul_left a r r;
-    assert (res == (((a * r) * r) / r) % n);
     multiple_division_lemma (a * r) r
 
 val lemma_mont_reduction:
@@ -264,29 +213,22 @@ val lemma_mod_exp_1:
                acc' % n == (a * acc / r) % n))
 	(ensures (res % n == ((pow a (2 * b2 + 1)) * acc / pow r (2 * b2 + 1)) % n))
 let lemma_mod_exp_1 n a a2 b b2 acc acc' r res =
+    assert (res % n == ((pow a2 b2) * acc' / pow r b2) % n);
     lemma_mod_exp n a a2 b b2 acc' r res;
-    assert (res % n == ((pow a (2 * b2)) * acc' / pow r (2 * b2)) % n);
     lemma_mod_mult_div acc' (pow a (2 * b2)) (pow r (2 * b2)) n;
-    assert (res % n == ((pow a (2 * b2)) * ((a * acc / r) % n) / pow r (2 * b2)) % n);
     lemma_mod_mult_div (a * acc / r) (pow a (2 * b2)) (pow r (2 * b2)) n;
-    //assert (res % n == (((pow a (2 * b2)) * (a * acc / r)) / pow r (2 * b2)) % n);
     lemma_mod_mult_div_1 ((pow a (2 * b2)) * (a * acc / r)) (pow r (2 * b2)) n;
-    assert (res % n == ((((pow a (2 * b2)) * (a * acc / r)) % n) / pow r (2 * b2)) % n);
     lemma_mult_div_mod (pow a (2 * b2)) (a * acc) r n;
-    assert (res % n == ((((pow a (2 * b2)) * (a * acc) / r) % n) / pow r (2 * b2)) % n);
     lemma_mod_mult_div_1 ((pow a (2 * b2)) * (a * acc) / r) ( pow r (2 * b2)) n;
-    assert (res % n == (((pow a (2 * b2)) * (a * acc) / r) / pow r (2 * b2)) % n);
     division_multiplication_lemma ((pow a (2 * b2)) * (a * acc)) r (pow r (2 * b2));
-    assert (res % n == (((pow a (2 * b2)) * (a * acc)) / (r * pow r (2 * b2))) % n);
     paren_mul_right (pow a (2 * b2)) a acc;
+    paren_mul_left (pow a (2 * b2)) a acc;
     assert_norm (pow a 1 = a);
     lemma_pow a 1 (2 * b2);
-    assert (a * pow a (2 * b2) = pow a (2 * b2 + 1));
     assert_norm (pow r 1 = r);
-    lemma_pow r 1 (2 * b2);
-    assert (r * pow r (2 * b2) = pow r (2 * b2 + 1))
+    lemma_pow r 1 (2 * b2)
 
-#reset-options "--z3rlimit 150 --max_fuel 0"
+#reset-options "--z3rlimit 300 --max_fuel 0"
 
 val lemma_mod_exp_2:
 	n:nat{n > 1} -> a:nat -> a_r:nat ->
@@ -295,14 +237,14 @@ val lemma_mod_exp_2:
                res_r % n == ((pow a_r b) * acc_r / pow r b) % n))
 	(ensures (res_r % n == ((pow a b) * r) % n))
 let lemma_mod_exp_2 n a a_r b acc_r r res_r =
+    assert (res_r % n == ((pow a_r b) * acc_r / pow r b) % n);
     lemma_mod_mult_div (pow a_r b) acc_r (pow r b) n;
     assert (res_r % n == (((pow a_r b) % n) * acc_r / pow r b) % n);
     lemma_pow_mod a_r b n;
     assert ((pow a_r b) % n == (pow ((a * r) % n) b) % n);
-    lemma_pow_mod (a * r) b n;  
+    lemma_pow_mod (a * r) b n;
     assert ((pow a_r b) % n == (pow (a * r) b) % n);
     lemma_pow_mul a r b;
-    assert ((pow a_r b) % n == ((pow a b) * (pow r b)) % n);
     assert (res_r % n == ((((pow a b) * (pow r b)) % n) * acc_r / pow r b) % n);
     lemma_mod_mult_div ((pow a b) * (pow r b)) acc_r (pow r b) n;
     assert (res_r % n == (((pow a b) * (pow r b) * acc_r) / pow r b) % n);
@@ -311,3 +253,158 @@ let lemma_mod_exp_2 n a a_r b acc_r r res_r =
     lemma_mod_mul_distr_l acc_r (pow a b) n;
     lemma_mod_mul_distr_l r (pow a b) n;
     assert (res_r % n == (r * pow a b) % n)
+
+(* LEMMAS for exponent blinding *)
+val lemma_mod_pq:
+    a:nat -> b:nat -> p:nat{p > 1} -> q:nat{q > 1} -> Lemma
+    (requires (a % p == b % p /\ a % q == b % q))
+    (ensures (a % (p * q) == b % (p * q)))
+let lemma_mod_pq a b p q = admit()
+
+// m ^ (p - 1) = 1 (mod p) where gcd(m, p) = 1 and p is a prime number
+val fermat_little_theorem:
+    p:nat{p > 1} -> m:nat{m > 0} -> Lemma
+    (requires (m % p <> 0))
+    (ensures ((pow m (p - 1)) % p == 1))
+let fermat_little_theorem p m = admit()
+
+val lemma_exp_blinding_q:
+    n:nat{n > 1} -> phi_n:nat -> p:elem n{p > 1} ->
+    q:elem n{q > 1} -> m:elem n{m > 0} -> Lemma
+    (requires (phi_n == (p - 1) * (q - 1) /\ n = p * q /\ m % q <> 0))
+    (ensures ((pow m phi_n) % q == 1))
+let lemma_exp_blinding_q n phi_n p q m =
+    let res = (pow m phi_n) % q in
+    lemma_pow_pow m (q - 1) (p - 1);
+    lemma_pow_mod (pow m (q - 1)) (p - 1) q;
+    fermat_little_theorem q m;
+    lemma_pow_1 (p - 1)
+
+val lemma_exp_blinding_pq:
+    n:nat{n > 1} -> phi_n:nat -> p:elem n{p > 1} ->
+    q:elem n{q > 1} -> m:elem n{m > 0} -> Lemma
+    (requires (phi_n == (p - 1) * (q - 1) /\ n = p * q /\ m % p <> 0 /\ m % q <> 0))
+    (ensures ((pow m phi_n) % (p * q) == 1))
+let lemma_exp_blinding_pq n phi_n p q m =
+    lemma_exp_blinding_q n phi_n p q m;
+    lemma_exp_blinding_q n phi_n q p m;
+    small_modulo_lemma_1 1 p;
+    small_modulo_lemma_1 1 q;
+    lemma_mod_pq (pow m phi_n) 1 p q;
+    small_modulo_lemma_1 1 n
+
+#reset-options "--z3rlimit 150 --max_fuel 0"
+
+val lemma_exp_blinding_1:
+    n:nat{n > 1} -> phi_n:nat -> p:elem n{p > 1} -> q:elem n{q > 1} ->
+    d:elem n{d > 0} -> m:elem n{m > 0} -> r:nat -> Lemma
+    (requires (phi_n = (p - 1) * (q - 1) /\ n = p * q /\ m % p <> 0 /\ m % q <> 0))
+    (ensures ((pow m (d + r * phi_n)) % n  == (pow m d) % n))
+let lemma_exp_blinding_1 n phi_n p q d m r =
+    let res:nat = (pow m (d + r * phi_n)) % n in
+    lemma_pow m d (r * phi_n);
+    lemma_pow_pow m phi_n r;
+    lemma_pow_mod (pow m phi_n) r n;
+    assert ((pow (pow m phi_n) r) % n == (pow ((pow m phi_n) % n) r) % n);
+    lemma_exp_blinding_pq n phi_n p q m;
+    assert ((pow m phi_n) % (p * q) == 1);
+    assert ((pow (pow m phi_n) r) % n == (pow 1 r) % n);
+    lemma_pow_1 r;
+    modulo_lemma 1 n;
+    lemma_mod_mul_distr_l (pow m (r * phi_n)) (pow m d) n;
+    assert (((pow m (d + r * phi_n)) % n  == (pow m d) % n))
+
+val lemma_exp_blinding_0_q0:
+    n:nat{n > 1} -> phi_n:nat -> p:elem n{p > 1} -> q:elem n{q > 1} ->
+    d:elem n{d > 0} -> m:elem n{m > 0} -> r:nat -> Lemma
+    (requires (phi_n = (p - 1) * (q - 1) /\ n = p * q /\ m % q = 0))
+    (ensures ((pow m (d + r * phi_n)) % q == (pow m d) % q))
+let lemma_exp_blinding_0_q0 n phi_n p q d m r =
+    let res:nat = pow m (d + r * phi_n) in
+    assert (res % q == (pow m (d + r * phi_n)) % q);
+    lemma_pow_mod m (d + r * phi_n) q;
+    lemma_pow_0 (d + r * phi_n);
+    lemma_pow_mod m d q;
+    lemma_pow_0 d
+
+#reset-options "--z3rlimit 300 --max_fuel 0"
+
+val lemma_exp_blinding_0_q1:
+    n:nat{n > 1} -> phi_n:nat -> p:elem n{p > 1} -> q:elem n{q > 1} ->
+    d:elem n{d > 0} -> m:elem n{m > 0} -> r:nat -> Lemma
+    (requires (phi_n = (p - 1) * (q - 1) /\ n = p * q /\ m % p <> 0))
+    (ensures ((pow m (d + r * phi_n)) % p == (pow m d) % p))
+let lemma_exp_blinding_0_q1 n phi_n p q d m r =
+    lemma_exp_blinding_q n phi_n q p m;
+    assert ((pow m phi_n) % p == 1);
+    let res:nat = pow m (d + r * phi_n) in
+    assert (res % p == (pow m (d + r * phi_n)) % p);
+    lemma_pow m d (r * phi_n);
+    assert (res % p == ((pow m d) * (pow m (r * phi_n))) % p);
+    lemma_pow_pow m phi_n r;
+    lemma_pow_mod (pow m phi_n) r p;
+    assert ((pow (pow m phi_n) r) % p == (pow ((pow m phi_n) % p) r) % p);
+    assert ((pow (pow m phi_n) r) % p == (pow 1 r) % p);
+    lemma_pow_1 r;
+    modulo_lemma 1 p;
+    lemma_mod_mul_distr_l (pow m (r * phi_n)) (pow m d) p
+
+val lemma_exp_blinding_0_q:
+    n:nat{n > 1} -> phi_n:nat -> p:elem n{p > 1} -> q:elem n{q > 1} ->
+    d:elem n{d > 0} -> m:elem n{m > 0} -> r:nat -> Lemma
+    (requires (phi_n = (p - 1) * (q - 1) /\ n = p * q /\ m % q = 0 /\ m % p <> 0))
+    (ensures ((pow m (d + r * phi_n)) % n == (pow m d) % n))
+let lemma_exp_blinding_0_q n phi_n p q d m r =
+    let res:nat = pow m (d + r * phi_n) in
+    lemma_exp_blinding_0_q0 n phi_n p q d m r;
+    lemma_exp_blinding_0_q1 n phi_n p q d m r;
+    lemma_mod_pq res (pow m d) p q;
+    assert (res % n == (pow m d) % n)
+
+val lemma_exp_blinding_0_pq:
+    n:nat{n > 1} -> phi_n:nat -> p:elem n{p > 1} -> q:elem n{q > 1} ->
+    d:elem n{d > 0} -> m:elem n -> r:nat -> Lemma
+    (requires (phi_n = (p - 1) * (q - 1) /\ n = p * q /\ m % q = 0 /\ m % p = 0))
+    (ensures ((pow m (d + r * phi_n)) % n == (pow m d) % n))
+let lemma_exp_blinding_0_pq n phi_n p q d m r =
+    small_modulo_lemma_1 0 p;
+    small_modulo_lemma_1 0 q;
+    lemma_mod_pq m 0 p q;
+    small_modulo_lemma_1 0 n;
+    assert (m % n == 0);
+    small_modulo_lemma_1 m n;
+    assert (m = 0);
+    lemma_pow_0 (d + r * phi_n);
+    lemma_pow_0 d
+
+val lemma_exp_blinding_0:
+    n:nat{n > 1} -> phi_n:nat -> p:elem n{p > 1} -> q:elem n{q > 1} ->
+    d:elem n{d > 0} -> m:elem n -> r:nat -> Lemma
+    (requires (phi_n = (p - 1) * (q - 1) /\ n = p * q /\ 
+                (m = 0 \/ m % p = 0 \/ m % q = 0)))
+    (ensures ((pow m (d + r * phi_n)) % n  == (pow m d) % n))
+let lemma_exp_blinding_0 n phi_n p q d m r =
+    if (m = 0) then begin
+        lemma_pow_0 (d + r * phi_n);
+        lemma_pow_0 d end
+    else begin
+        if (m % p = 0 && m % q <> 0) then
+            lemma_exp_blinding_0_q n phi_n q p d m r
+        else begin
+            if (m % q = 0 && m % p <> 0) then
+                lemma_exp_blinding_0_q n phi_n p q d m r
+                else begin
+                    assert (m % p = 0 && m % q = 0);
+                    lemma_exp_blinding_0_pq n phi_n p q d m r end
+            end
+        end
+
+val lemma_exp_blinding:
+    n:nat{n > 1} -> phi_n:nat -> p:elem n{p > 1} -> q:elem n{q > 1} ->
+    d:elem n{d > 0} -> m:elem n -> r:nat -> Lemma
+    (requires (phi_n = (p - 1) * (q - 1) /\ n = p * q))
+    (ensures ((pow m (d + r * phi_n)) % n  == (pow m d) % n))
+let lemma_exp_blinding n phi_n p q d m r =
+    if (m = 0 || m % p = 0 || m % q = 0) then 
+        lemma_exp_blinding_0 n phi_n p q d m r
+    else lemma_exp_blinding_1 n phi_n p q d m r
